doc-src/TutorialI/Types/Overloading2.thy
@@ -16,6 +16,35 @@ le_list_def: "xs <<= (ys::'a::ordrel list) \<equiv>
 
 text{*\noindent
 The infix function @{text"!"} yields the nth element of a list.
-%However, we retract the componetwise comparison of lists and return
-%Note: only one definition because based on name.
+*}
+
+subsubsection{*Predefined overloading*}
+
+text{*
+HOL comes with a number of overloaded constants and corresponding classes.
+The most important ones are listed in Table~\ref{tab:overloading}. They are
+defined on all numeric types and somtimes on other types as well, for example
+@{text"-"}, @{text"\<le>"} and @{text"<"} on sets.
+
+\begin{table}[htbp]
+\begin{center}
+\begin{tabular}{lll}
+Constant & Type & Syntax \\
+\hline
+@{term 0} & @{text "'a::zero"} \\
+@{text"+"} & @{text "('a::plus) \<Rightarrow> 'a \<Rightarrow> 'a"} & (infixl 65) \\
+@{text"-"} & @{text "('a::minus) \<Rightarrow> 'a \<Rightarrow> 'a"} &  (infixl 65) \\
+@{text"*"} & @{text "('a::times) \<Rightarrow> 'a \<Rightarrow> 'a"} & (infixl 70) \\
+@{text"^"} & @{text "('a::power) \<Rightarrow> nat \<Rightarrow> 'a"} & (infixr 80) \\
+@{text"-"} & @{text "('a::minus) \<Rightarrow> 'a"} \\
+@{term abs} &  @{text "('a::minus) \<Rightarrow> 'a"} \\
+@{text"\<le>"} & @{text "('a::ord) \<Rightarrow> 'a \<Rightarrow> bool"} & (infixl 50) \\
+@{text"<"} & @{text "('a::ord) \<Rightarrow> 'a \<Rightarrow> bool"} & (infixl 50) \\
+@{term min} &  @{text "('a::ord) \<Rightarrow> 'a \<Rightarrow> 'a"} \\
+@{term max} &  @{text "('a::ord) \<Rightarrow> 'a \<Rightarrow> 'a"} \\
+\end{tabular}
+\caption{Overloaded constants in HOL}
+\label{tab:overloading}
+\end{center}
+\end{table}
 *}(*<*)end(*>*)
